Changed terminology

theories/L6_PCPS/Heap/dead_param_elim.v
@@ -15,12 +15,12 @@ Open Scope ctx_scope.
 Open Scope fun_scope.
 Close Scope Z_scope.
 
-Inductive dropping_fun : Type := 
-| Dropping: list (list var) -> list (list bool) -> dropping_fun. 
+Inductive live_fun : Type := 
+| Live: list (list var) -> list (list bool) -> live_fun. 
 
-Fixpoint bool_drop (drop : dropping_fun) : list (list bool) := 
-match drop with
-| Dropping yss bss => bss
+Fixpoint bool_live (L : live_fun) : list (list bool) := 
+match L with
+| Live yss bss => bss
 end. 
 
 (* list of list of variables corresponding to list of fundefs *)
@@ -55,11 +55,11 @@ match B with
 | Fnil => []
 end. 
 
-(* Make initial dropping function *)
-Fixpoint get_drop_initial (B : fundefs) : dropping_fun := 
+(* Make initial Lping function *)
+Fixpoint get_live_initial (B : fundefs) : live_fun := 
 let yss := get_vars B  in
 let bss := get_bools B  in 
-(Dropping yss bss). 
+(Live yss bss). 
 
 Fixpoint contains (xs : list var) (y : var) : bool := 
 match xs with 
@@ -82,137 +82,137 @@ match funs with
 | f :: funs' => if (peq f x) then (true, n) else find_fun x funs' (n+1)
 end. 
 
-Fixpoint add_escaping (x : var) (drop : dropping_fun) (funs : list var) : dropping_fun :=
+Fixpoint add_escaping (x : var) (L : live_fun) (funs : list var) : live_fun :=
 let (b, n) := find_fun x funs 0 in
 if b then 
-  match drop with 
-  | Dropping yss bss =>
+  match L with 
+  | Live yss bss =>
     let ys := nth n yss [] in
     let bs := get_bool_true ys in
     let bss' := replace_nth n bss bs in
-    Dropping yss bss'
+    Live yss bss'
   end
-else drop. 
+else L. 
 
-Fixpoint add_escapings (xs : list var) (drop : dropping_fun) (funs : list var) (f : var) : dropping_fun :=
+Fixpoint add_escapings (xs : list var) (L : live_fun) (funs : list var) (f : var) : live_fun :=
 if contains funs f then 
 match xs with 
-| x :: xs' => add_escapings xs' (add_escaping x drop funs) funs f
-| [] => drop
+| x :: xs' => add_escapings xs' (add_escaping x L funs) funs f
+| [] => L
 end
-else drop. 
+else L. 
 
-Fixpoint add_escapings' (xs : list var) (drop : dropping_fun) (funs : list var) : dropping_fun :=
+Fixpoint add_escapings' (xs : list var) (L : live_fun) (funs : list var) : live_fun :=
 match xs with 
-| x :: xs' => add_escapings' xs' (add_escaping x drop funs) funs
-| [] => drop
+| x :: xs' => add_escapings' xs' (add_escaping x L funs) funs
+| [] => L
 end. 
 
-(* Find the relevant variable and undrop it if necessary *)
+(* Find the relevant variable and unL it if necessary *)
 Fixpoint add_var_helper (x : var) (ys : list var) (bs : list bool) : list bool := 
 match ys, bs with 
 | y :: ys', b :: bs' => if (peq x y) then (true :: bs') else (b :: (add_var_helper x ys' bs'))
 | _, _ => bs
 end. 
 
-(* Undrop a variable *)
-Fixpoint add_var (x : var) (drop : dropping_fun) (n : nat) : dropping_fun := 
-match drop with
-| Dropping yss bss => 
+(* UnL a variable *)
+Fixpoint add_var (x : var) (L : live_fun) (n : nat) : live_fun := 
+match L with
+| Live yss bss => 
   let ys := nth n yss [] in
   let bs := nth n bss [] in
   let bs' := add_var_helper x ys bs in
   let bss' := replace_nth n bss bs' in 
-  Dropping yss bss'
+  Live yss bss'
 end. 
 
-(* Undrop a list of variables *)
-Fixpoint add_vars (xs : list var) (drop : dropping_fun) (n : nat) : dropping_fun := 
+(* UnL a list of variables *)
+Fixpoint add_vars (xs : list var) (L : live_fun) (n : nat) : live_fun := 
 match xs with 
-| [] => drop
-| x :: xs' => add_vars xs' (add_var x drop n) n
+| [] => L
+| x :: xs' => add_vars xs' (add_var x L n) n
 end. 
 
-Fixpoint add_fun_args (n : nat) (xs : list var) (bs : list bool) (drop : dropping_fun) : dropping_fun :=
+Fixpoint add_fun_args (n : nat) (xs : list var) (bs : list bool) (L : live_fun) : live_fun :=
 match (xs, bs) with 
-| ([], []) => drop
+| ([], []) => L
 | (x :: xs', b :: bs') => 
-  if (eqb b true) then let drop' := add_var x drop n in add_fun_args n xs' bs' drop'
-  else add_fun_args n xs' bs' drop
-| _ => drop
+  if (eqb b true) then let L' := add_var x L n in add_fun_args n xs' bs' L'
+  else add_fun_args n xs' bs' L
+| _ => L
 end. 
 
-Fixpoint add_fun_vars (f : var) (funs : list var) (xs : list var) (drop : dropping_fun) (m : nat) : dropping_fun :=
+Fixpoint add_fun_vars (f : var) (funs : list var) (xs : list var) (L : live_fun) (m : nat) : live_fun :=
 let (b, n) := find_fun f funs 0 in
 if b then (
-  let bss := bool_drop drop in
+  let bss := bool_live L in
   let bs := nth n bss [] in
-  add_fun_args m xs bs drop
+  add_fun_args m xs bs L
 )
-else add_vars xs drop m. 
+else add_vars xs L m. 
 
-Fixpoint escaping_fun_exp (e : exp) (drop : dropping_fun) (funs : list var) := 
+Fixpoint escaping_fun_exp (e : exp) (L : live_fun) (funs : list var) := 
 match e with 
 | Eapp f t ys =>
-  add_escapings' ys drop funs 
-| Econstr x t ys e' => escaping_fun_exp e' (add_escapings' ys drop funs) funs 
-| Eproj x t n y e' => escaping_fun_exp e' drop funs
+  add_escapings' ys L funs 
+| Econstr x t ys e' => escaping_fun_exp e' (add_escapings' ys L funs) funs 
+| Eproj x t n y e' => escaping_fun_exp e' L funs
 | Ecase x P => 
-  (fix mapM_LD (l : list (cTag * exp)) (drop : dropping_fun) := 
+  (fix mapM_LD (l : list (cTag * exp)) (L : live_fun) := 
   match l with 
-  | [] => drop
+  | [] => L
   | (c', e') :: l' =>
-    let drop' := escaping_fun_exp e' drop funs in mapM_LD l' drop'
-  end) P drop
-| Ehalt x => drop
-| Efun fl e' => drop
-| Eprim x fs ys e' => escaping_fun_exp e' drop funs
+    let L' := escaping_fun_exp e' L funs in mapM_LD l' L'
+  end) P L
+| Ehalt x => add_escaping x L funs
+| Efun fl e' => L
+| Eprim x fs ys e' => escaping_fun_exp e' L funs
 end. 
 
-Fixpoint escaping_fun_fundefs (B : fundefs) (drop : dropping_fun) (funs : list var) := 
+Fixpoint escaping_fun_fundefs (B : fundefs) (L : live_fun) (funs : list var) := 
 match B with 
 | Fcons f ft xs e B' => 
-  let drop' := escaping_fun_exp e drop funs in
-  escaping_fun_fundefs B' drop' funs
-| Fnil => drop
+  let L' := escaping_fun_exp e L funs in
+  escaping_fun_fundefs B' L' funs
+| Fnil => L
 end. 
 
-Fixpoint live_expr (B : fundefs) (drop : dropping_fun) (funs : list var) (n : nat) (e : exp) : dropping_fun := 
+Fixpoint live_expr (B : fundefs) (L : live_fun) (funs : list var) (n : nat) (e : exp) : live_fun := 
 match e with 
 | Econstr x t ys e' => 
-  let drop' := add_vars ys drop n in
-  live_expr B drop' funs n e'
+  let L' := add_vars ys L n in
+  live_expr B L' funs n e'
 | Eproj x t m y e' => 
-  let drop' := add_var y drop n in
-  live_expr B drop' funs n e'
+  let L' := add_var y L n in
+  live_expr B L' funs n e'
 | Ecase x P => 
-  let drop' := add_var x drop n in
-  (fix mapM_LD  (l : list (cTag * exp))  (drop : dropping_fun) := 
+  let L' := add_var x L n in
+  (fix mapM_LD  (l : list (cTag * exp))  (L : live_fun) := 
   match l with 
-  | [] => drop
+  | [] => L
   | (c', e') :: l'=>
-    let drop' := live_expr B drop funs n e' in
-    mapM_LD l' drop'
-  end) P drop'
-| Ehalt x => add_var x drop n 
+    let L' := live_expr B L funs n e' in
+    mapM_LD l' L'
+  end) P L'
+| Ehalt x => add_var x L n 
 | Eapp f t ys =>  
-  let drop' := add_var f drop n in
-  let drop'' := add_fun_vars f funs ys drop' n in
-  drop''
-| Efun fl e' => drop
+  let L' := add_var f L n in
+  let L'' := add_fun_vars f funs ys L' n in
+  L''
+| Efun fl e' => L
 | Eprim x f ys e' =>  
-  let drop' := add_var f drop n in
-  let drop'' := add_vars ys drop' n in
-  live_expr B drop'' funs n e'
+  let L' := add_var f L n in
+  let L'' := add_vars ys L' n in
+  live_expr B L'' funs n e'
 end. 
 
-(* One pass through fundefs to drop variables and keep track of live variables *)
-Fixpoint live (B : fundefs) (drop : dropping_fun) (funs : list var) (n : nat) : dropping_fun := 
+(* One pass through fundefs to L variables and keep track of live variables *)
+Fixpoint live (B : fundefs) (L : live_fun) (funs : list var) (n : nat) : live_fun := 
 match B with 
 | Fcons f ft xs e B' => 
-  let drop' := live_expr B drop funs n e in
-  live B' drop' funs (n+1)
-| Fnil => drop
+  let L' := live_expr B L funs n e in
+  live B' L' funs (n+1)
+| Fnil => L
 end. 
 
 Fixpoint check_list_equality (l1 : list bool) (l2 : list bool) : bool := 
@@ -229,9 +229,9 @@ match (l1, l2) with
 | _ => false
 end. 
 
-Fixpoint drop_equality (drop1: dropping_fun) (drop2 : dropping_fun) : bool := 
-match (drop1, drop2) with
-|(Dropping yss1 bss1, Dropping yss2 bss2) =>
+Fixpoint live_equality (L1: live_fun) (L2 : live_fun) : bool := 
+match (L1, L2) with
+|(Live yss1 bss1, Live yss2 bss2) =>
   check_list_list_equality bss1 bss2
 end. 
 
@@ -241,82 +241,82 @@ match B with
 | Fnil => n
 end. 
 
-(* Inductively create dropping functions for B, when they are equal, stop *)
+(* Inductively create Lping functions for B, when they are equal, stop *)
 (* Note that a naive upper bound for the number of passes is the number of total variables
-   as at each step, if the process doesn't terminate at least one variable must be dropped *)
-Fixpoint find_drop_helper (B : fundefs) (prev_drop : dropping_fun) (funs : list var) (n : nat) : dropping_fun := 
+   as at each step, if the process doesn't terminate at least one variable must be Lped *)
+Fixpoint find_live_helper (B : fundefs) (prev_L : live_fun) (funs : list var) (n : nat) : live_fun := 
 match n with 
-| 0 => prev_drop
+| 0 => prev_L
 | S n' => 
-  let curr_drop := live B prev_drop funs 0 in 
-  if (drop_equality prev_drop curr_drop) then prev_drop
-  else find_drop_helper B curr_drop funs n'
-end.
+  let curr_L := live B prev_L funs 0 in 
+  if (live_equality prev_L curr_L) then prev_L
+  else find_live_helper B curr_L funs n'
+end. 
 
-Fixpoint find_drop (e : exp) : dropping_fun := 
+Fixpoint find_live (e : exp) : live_fun := 
 match e with 
 | Efun B e' =>
   let funs := get_funs B in
-  let initial_drop := get_drop_initial B in
-  let drop' := escaping_fun_exp e' (escaping_fun_fundefs B initial_drop funs) funs in
+  let initial_L := get_live_initial B in
+  let L' := escaping_fun_exp e' (escaping_fun_fundefs B initial_L funs) funs in
   let n := num_vars B 0 in
-  (* initial_drop *)
-  (* drop' *)
-  find_drop_helper B drop' funs n
-| _ => Dropping [[]] [[]]
+  (* initial_L *)
+  (* L' *)
+  find_live_helper B L' funs n
+| _ => Live [[]] [[]]
 end. 
 
-Fixpoint drop_args (ys : list var) (bs : list bool) : list var := 
+Fixpoint live_args (ys : list var) (bs : list bool) : list var := 
 match ys, bs with 
 | [], [] => ys
 | y :: ys', b :: bs' => 
-  if (eqb b true) then y :: (drop_args ys' bs')
-  else drop_args ys' bs'
+  if (eqb b true) then y :: (live_args ys' bs')
+  else live_args ys' bs'
 | _, _ => ys
 end. 
 
-Fixpoint dropper_expr (drop : dropping_fun) (funs : list var) (e : exp) : exp := 
+Fixpoint eliminate_expr (L : live_fun) (funs : list var) (e : exp) : exp := 
 match e with 
-| Econstr x t ys e' => Econstr x t ys (dropper_expr drop funs e')
-| Eproj x t m y e' => Eproj x t m y (dropper_expr drop funs e')
+| Econstr x t ys e' => Econstr x t ys (eliminate_expr L funs e')
+| Eproj x t m y e' => Eproj x t m y (eliminate_expr L funs e')
 | Ecase x P =>
   let P' := (fix mapM_LD (l : list (cTag * exp)) : list (cTag * exp) :=
   match l with 
   | [] => l
-  | (c', e') :: l' => (c', dropper_expr drop funs e') :: mapM_LD l'
+  | (c', e') :: l' => (c', eliminate_expr L funs e') :: mapM_LD l'
   end) P in
   Ecase x P'
 | Ehalt x => Ehalt x
 | Efun fl e' => e
-| Eprim x f ys e' => Eprim x f ys (dropper_expr drop funs e')
+| Eprim x f ys e' => Eprim x f ys (eliminate_expr L funs e')
 | Eapp f t ys => 
   let (b, n) := find_fun f funs 0 in
   if b then (
-    let bss := bool_drop drop in
-    let ys' := drop_args ys (nth n bss []) in
+    let bss := bool_live L in
+    let ys' := live_args ys (nth n bss []) in
     Eapp f t ys')
   else Eapp f t ys
 end. 
 
-Fixpoint dropper_fundefs (B : fundefs) (drop : dropping_fun) (funs : list var) (n : nat) := 
-match drop with 
-| Dropping yss bss =>
+Fixpoint eliminate_fundefs (B : fundefs) (L : live_fun) (funs : list var) (n : nat) := 
+match L with 
+| Live yss bss =>
   match B with 
   | Fcons f ft ys e B' => 
-    let ys' := drop_args ys (nth n bss []) in
-    let e' := dropper_expr drop funs e in
-    Fcons f ft ys' e' (dropper_fundefs B' drop funs (n + 1))
+    let ys' := live_args ys (nth n bss []) in
+    let e' := eliminate_expr L funs e in
+    Fcons f ft ys' e' (eliminate_fundefs B' L funs (n + 1))
   | Fnil => B
   end 
 end. 
 
-Fixpoint dropper (e : exp) : exp := 
+Fixpoint eliminate (e : exp) : exp := 
 match e with 
 | Efun B e' =>
   let funs := get_funs B in
-  let drop := find_drop e in 
-  let B' := dropper_fundefs B drop funs 0 in
-  let e'' := dropper_expr drop funs e' in
+  let L := find_live e in 
+  let B' := eliminate_fundefs B L funs 0 in
+  let e'' := eliminate_expr L funs e' in
   Efun B' e''
 | _ => e
 end. 
