theories/L6_PCPS/Heap/dead_param_elim_rel.v
@@ -1,5 +1,5 @@
-(* Correctness proof for lambda lifting. Part of the CertiCoq project.
- * Author: Zoe Paraskevopoulou, 2016
+(* Relation for Dead Parameter Elimination. Part of the CertiCoq project.
+ * Author: Katja Vassilev, 2019
  *)
 
 Require Import L6.cps L6.cps_util L6.set_util L6.hoisting L6.identifiers L6.ctx
@@ -15,123 +15,100 @@ Open Scope ctx_scope.
 Open Scope fun_scope.
 Close Scope Z_scope.
 
-Fixpoint check_list_equality (l1 : list var) (l2 : list var) : bool := 
-match (l1, l2) with 
-| ([], []) => true
-| (hd1 :: tl1, hd2 :: tl2) => if (peq hd1 hd2) then check_list_equality tl1 tl2 else false 
-| _ => false
-end. 
-
-Fixpoint drop_args (ys : list var) (bs : list bool) : list var := 
-match ys, bs with 
-| [], [] => ys
-|y :: ys', b :: bs' => 
-  if (eqb b true) then y :: (drop_args ys' bs')
-  else drop_args ys' bs'
-| _, _ => ys
-end. 
-(* 
-Fixpoint Drop_args (ys : list var) (bs : list bool) (ys' : list var) : Prop := 
-let xs' := drop_args ys bs in
-if check_list_equality xs' ys' then True
-else False. 
- *)
-
-
 (* S is the set of the dropped parameters of the function we're in. We need it
    to make sure that these are not used anywhere in the program, and so the proof will go through.
    Everything that we want to keep we want to make sure that is not in S.
-   the list of booleans is the drop parameters of the function we are calling and we need it so that
+   the list of booleans is the L parameters of the function we are calling and we need it so that
    the application has the right arity.
  *)
-Inductive Drop_args (S : Ensemble var) : list var -> list bool -> list var -> Prop :=
-| ADrop_nil : Drop_args S [] [] []
-| ADrop_cons_drop :
+Inductive Live_args (S : Ensemble var) : list var -> list bool -> list var -> Prop :=
+| ALive_nil : Live_args S [] [] []
+| ALive_cons_L :
     forall (x : var) (xs : list var) (bs: list bool) (ys : list var),
-      Drop_args S xs bs ys ->
-      Drop_args S (x :: xs) (false :: bs) ys
-| ADrop_cons_keep :
+      Live_args S xs bs ys ->
+      Live_args S (x :: xs) (false :: bs) ys
+| ALive_cons_keep :
     forall (x : var) (xs : list var) (bs: list bool) (ys : list var),
-      Drop_args S xs bs ys ->
+      Live_args S xs bs ys ->
       ~ x \in S -> 
-      Drop_args S (x :: xs) (true :: bs) (x :: ys).
+      Live_args S (x :: xs) (true :: bs) (x :: ys).
 
-Definition dropped_funs drop : Ensemble var :=
-  [set f | exists bs, drop f = Some bs /\ Exists (fun x => x = false) bs]. 
+Definition eliminated_funs L : Ensemble var :=
+  [set f | exists bs, L f = Some bs /\ Exists (fun x => x = false) bs]. 
 
 (* S is the set of formal parameters that have been dropped from the *current* function.
    That is, whatever is in S, is undefined in the environment when we execute the code. *)
-Inductive Drop_body (drop : var -> option (list bool)) (S : Ensemble var) :  exp -> exp -> Prop := 
-| BDrop_Constr : 
+Inductive Live_body (L : var -> option (list bool)) (S : Ensemble var) :  exp -> exp -> Prop := 
+| BLive_Constr : 
   forall (x : var) (ys : list var) (ct : cTag) (e : exp) (e' : exp), 
-    Disjoint _ (FromList ys) (S :|: dropped_funs drop) -> 
-    Drop_body drop S e e' ->
-    Drop_body drop S (Econstr x ct ys e) (Econstr x ct ys e')
-| BDrop_Prim : 
+    Disjoint _ (FromList ys) (S :|: eliminated_funs L) -> 
+    Live_body L S e e' ->
+    Live_body L S (Econstr x ct ys e) (Econstr x ct ys e')
+| BLive_Prim : 
   forall (x : var) (g : prim) (ys : list var) (e : exp) (e' : exp), 
-    Disjoint _ (FromList ys) (S :|: dropped_funs drop) -> 
-    Drop_body drop S e e' ->
-    Drop_body drop S (Eprim x g ys e) (Eprim x g ys e')
-| BDrop_Proj : 
+    Disjoint _ (FromList ys) (S :|: eliminated_funs L) -> 
+    Live_body L S e e' ->
+    Live_body L S (Eprim x g ys e) (Eprim x g ys e')
+| BLive_Proj : 
   forall (x : var) (ct : cTag) (n : N) (y : var) (e : exp) (e' : exp), 
-    ~ y \in (S :|: dropped_funs drop) ->
-    Drop_body drop S e e' ->
-    Drop_body drop S (Eproj x ct n y e) (Eproj x ct n y e')
-| BDrop_Case: 
+    ~ y \in (S :|: eliminated_funs L) ->
+    Live_body L S e e' ->
+    Live_body L S (Eproj x ct n y e) (Eproj x ct n y e')
+| BLive_Case: 
   forall (x : var) (ce : list (cTag * exp)) (ce' : list (cTag * exp)),
-    ~ x \in (S :|: dropped_funs drop) ->
-    Forall2 (fun p1 p2 => fst p1 = fst p2 /\ Drop_body drop S (snd p1) (snd p2)) ce ce' -> 
-    Drop_body drop S (Ecase x ce) (Ecase x ce')
-| BDrop_Halt : 
+    ~ x \in (S :|: eliminated_funs L) ->
+    Forall2 (fun p1 p2 => fst p1 = fst p2 /\ Live_body L S (snd p1) (snd p2)) ce ce' -> 
+    Live_body L S (Ecase x ce) (Ecase x ce')
+| BLive_Halt : 
     forall (x : var),
-      ~ x \in (S :|: dropped_funs drop) ->
-      Drop_body drop S (Ehalt x) (Ehalt x)
-| BDrop_App_Unknown :
+      ~ x \in (S :|: eliminated_funs L) ->
+      Live_body L S (Ehalt x) (Ehalt x)
+| BLive_App_Unknown :
     forall (f : var) (ys : list var) (ft : fTag),
       (* Unknown function application, f is not in the list of top-level
          function definitions. Therefore, it must be a parameter of the current
          function *)
-      ~ f \in (S :|: dropped_funs drop) ->
-      Disjoint _ (FromList ys) (S :|: dropped_funs drop) -> 
-      drop f = None -> 
-      Drop_body drop S (Eapp f ft ys) (Eapp f ft ys)
-| BDrop_App_Known :
+      ~ f \in (S :|: eliminated_funs L) ->
+      Disjoint _ (FromList ys) (S :|: eliminated_funs L) -> 
+      L f = None -> 
+      Live_body L S (Eapp f ft ys) (Eapp f ft ys)
+| BLive_App_Known :
     forall (f : var) (ys : list var) (ys' : list var) (ft : fTag) (bs : list bool),
-      drop f = Some bs ->
+      L f = Some bs ->
       ~ f \in S ->
-      Drop_args (S :|: dropped_funs drop) ys bs ys' ->
-      Drop_body drop S (Eapp f ft ys) (Eapp f ft ys').
+      Live_args (S :|: eliminated_funs L) ys bs ys' ->
+      Live_body L S (Eapp f ft ys) (Eapp f ft ys'). 
 
   
-Inductive Drop_params : list var -> list bool -> list var -> Ensemble var -> Prop :=
-| PDrop_nil : Drop_params [] [] [] (Empty_set _)
-| PDrop_cons_drop :
+Inductive Live_params : list var -> list bool -> list var -> Ensemble var -> Prop :=
+| PLive_nil : Live_params [] [] [] (Empty_set _)
+| PLive_cons_L :
     forall (x : var) (xs : list var) (bs: list bool) (ys : list var) (S : Ensemble var),
-      Drop_params xs bs ys S ->
-      Drop_params (x :: xs) (false :: bs) ys (x |: S)
-| PDrop_cons_keep :
+      Live_params xs bs ys S ->
+      Live_params (x :: xs) (false :: bs) ys (x |: S)
+| PLive_cons_keep :
     forall (x : var) (xs : list var) (bs: list bool) (ys : list var) (S : Ensemble var),
-      Drop_params xs bs ys S ->
-      Drop_params (x :: xs) (true :: bs) (x :: ys) S.
+      Live_params xs bs ys S ->
+      Live_params (x :: xs) (true :: bs) (x :: ys) S. 
+ 
 
-
-Inductive Drop_fundefs (drop : var -> option (list bool)) : fundefs -> fundefs -> Prop := 
-| FDrop_nil : 
-  Drop_fundefs drop Fnil Fnil
-| FDrop_cons : 
+Inductive Live_fundefs (L : var -> option (list bool)) : fundefs -> fundefs -> Prop := 
+| FLive_nil : 
+  Live_fundefs L Fnil Fnil
+| FLive_cons : 
   forall (F : fundefs) (F' : fundefs) (e : exp) (e' : exp) (xs ys : list var) (bs : list bool)
     (g : var) (ft : fTag) (S : Ensemble var), 
-    drop g = Some bs ->  
-    Drop_params xs bs ys S -> 
-    Drop_body drop S e e' ->
-    Drop_fundefs drop F F' ->
-    Drop_fundefs drop (Fcons g ft xs e F) (Fcons g ft ys e' F'). 
+    L g = Some bs ->  
+    Live_params xs bs ys S -> 
+    Live_body L S e e' ->
+    Live_fundefs L F F' ->
+    Live_fundefs L (Fcons g ft xs e F) (Fcons g ft ys e' F'). 
 
 
-Inductive Drop (drop : var -> option (list bool)) : fundefs -> exp -> fundefs -> exp -> Prop := 
-| Drop_toplevel :
+Inductive Live (L : var -> option (list bool)) : fundefs -> exp -> fundefs -> exp -> Prop := 
+| Live_toplevel :
     forall B e B' e',
-      domain drop <--> name_in_fundefs B -> (* XXX New *)
-      Drop_fundefs drop B B' ->
-      Drop_body drop (Empty_set _) e e' -> 
-      Drop drop B e B' e'. 
+      domain L <--> name_in_fundefs B -> (* XXX New *)
+      Live_fundefs L B B' ->
+      Live_body L (Empty_set _) e e' -> 
+      Live L B e B' e'. 
